Feedback

src/lib/communication/DY.Lib.Communication.Core.Properties.fst
@@ -1,4 +1,4 @@
-module DY.Lib.Communication.Properties
+module DY.Lib.Communication.Core.Properties
 
 open Comparse
 open DY.Core
@@ -12,9 +12,6 @@ open DY.Lib.State.Typed
 open DY.Lib.Communication.Core
 open DY.Lib.Communication.Core.Invariants
 open DY.Lib.Communication.Core.Lemmas
-
-open DY.Lib.Communication.RequestResponse
-open DY.Lib.Communication.RequestResponse.Invariants
 
 #set-options "--fuel 0 --ifuel 0 --z3rlimit 10 --z3cliopt 'smt.qi.eager_threshold=100'"
 
@@ -63,47 +60,3 @@ val sender_confauth_authentication:
     is_corrupt (prefix tr i) (long_term_key_label sender)
   )
 let sender_confauth_authentication #invs #a tr i higher_layer_preds sender receiver secret = ()
-
-
-(*** Request Response Pair Properties ***)
-
-val server_authentication:
-  {|protocol_invariants|} ->
-  #a:Type -> {| parseable_serializeable bytes a |} ->
-  tr:trace -> i:timestamp ->
-  higher_layer_resreq_preds:comm_reqres_higher_layer_event_preds a ->
-  client:principal -> server:principal -> payload:bytes -> key:bytes ->
-  Lemma
-  (requires
-    trace_invariant tr /\
-    has_communication_layer_reqres_event_predicates request_response_event_preconditions higher_layer_resreq_preds /\
-    event_triggered_at tr i client (CommClientReceiveResponse client server  payload key)    
-  )
-  (ensures
-    event_triggered (prefix tr i) server (CommServerSendResponse server payload) \/
-    is_corrupt (prefix tr i) (principal_label client) \/ 
-    is_corrupt (prefix tr i) (principal_label server)
-  )
-let server_authentication #invs #a tr i higher_layer_resreq_preds client server payload key = ()
-
-val key_secrecy_client:
-  {|protocol_invariants|} ->
-  tr:trace ->
-  client:principal -> server:principal ->
-  key:bytes -> payload:bytes -> 
-  Lemma
-  (requires
-    trace_invariant tr /\
-    has_communication_layer_state_predicates /\
-    attacker_knows tr key /\
-    (
-      (exists sid. state_was_set tr client sid (ClientSendRequest {server; payload; key})) \/
-      (exists sid. state_was_set tr client sid (ClientReceiveResponse {server; payload; key}))
-    )
-  )
-  (ensures
-    is_corrupt tr (principal_label client) \/ is_corrupt tr (principal_label server)
-  )
-let key_secrecy_client tr client server key payload =
-  attacker_only_knows_publishable_values tr key;
-  ()
