src/lib/communication/DY.Lib.Communication.RequestResponse.Invariants.fst
@@ -25,8 +25,8 @@ let aead_crypto_predicate_communication_layer #cusages = {
   pred = (fun tr key_usage key nonce msg ad ->
       (match parse authenticated_data ad with
       | None -> False
-      | Some {server} -> (
-        event_triggered tr server (CommServerSendResponse server msg)
+      | Some {server} -> (exists request.
+        event_triggered tr server (CommServerSendResponse server request msg)
       )
     )
   );
@@ -60,24 +60,24 @@ let has_communication_layer_reqres_crypto_predicates #cinvs =
 let state_predicates_communication_layer {|crypto_invariants|}: local_state_predicate communication_states = {
   pred = (fun tr prin sess_id st -> 
     match st with
-    | ClientSendRequest {server; payload; key} -> (
+    | ClientSendRequest {server; request; key} -> (
       let client = prin in
-      is_knowable_by (comm_label client server) tr payload /\
+      is_knowable_by (comm_label client server) tr request /\
       is_secret (comm_label client server) tr key /\
       key `has_usage tr` (AeadKey comm_layer_aead_tag empty)
     )
-    | ServerReceiveRequest {payload; key} -> (
+    | ServerReceiveRequest {request; key} -> (
       let server = prin in
       is_knowable_by (principal_label server) tr key /\
-      is_knowable_by (get_label tr key) tr payload /\
+      is_knowable_by (get_label tr key) tr request /\
       (
         key `has_usage tr` (AeadKey comm_layer_aead_tag empty) \/
         is_publishable tr key
       )
     )
-    | ClientReceiveResponse {server; payload; key} -> (
+    | ClientReceiveResponse {server; response; key} -> (
       let client = prin in
-      is_knowable_by (comm_label client server) tr payload /\
+      is_knowable_by (comm_label client server) tr response /\
       is_secret (comm_label client server) tr key
     )
   );
@@ -103,40 +103,41 @@ let has_communication_layer_state_predicates #invs =
 
 noeq
 type comm_reqres_higher_layer_event_preds (a:Type) {| parseable_serializeable bytes a |} = {
-  send_request: tr:trace -> client:principal -> server:principal -> payload:a -> key_label:label -> prop;
+  send_request: tr:trace -> client:principal -> server:principal -> request:a -> key_label:label -> prop;
   send_request_later:
     tr1:trace -> tr2:trace ->
-    client:principal -> server:principal -> payload:a -> key_label:label ->
+    client:principal -> server:principal -> request:a -> key_label:label ->
     Lemma
     (requires
-      send_request tr1 client server payload key_label /\
-      bytes_well_formed tr1 (serialize a payload) /\
+      send_request tr1 client server request key_label /\
+      bytes_well_formed tr1 (serialize a request) /\
       tr1 <$ tr2
     )
     (ensures
-      send_request tr2 client server payload key_label
+      send_request tr2 client server request key_label
     )
   ;
-  send_response: tr:trace -> server:principal -> payload:a -> prop;
+  send_response: tr:trace -> server:principal -> request:a -> response:a -> prop;
   send_response_later:
     tr1:trace -> tr2:trace ->
-    server:principal -> payload:a ->
+    server:principal -> request:a -> response:a ->
     Lemma
     (requires
-      send_response tr1 server payload /\
-      bytes_well_formed tr1 (serialize a payload) /\
+      send_response tr1 server request response /\
+      bytes_well_formed tr1 (serialize a request) /\
+      bytes_well_formed tr1 (serialize a response) /\
       tr1 <$ tr2
     )
     (ensures
-      send_response tr2 server payload
+      send_response tr2 server request response
     )
 }
 
 let default_comm_reqres_higher_layer_event_preds (a:Type) {| parseable_serializeable bytes a |} : comm_reqres_higher_layer_event_preds a = {
-  send_request = (fun tr client server payload key_label -> True);
-  send_request_later = (fun tr1 tr2 client server payload key_label -> ());
-  send_response = (fun tr server payload -> True);
-  send_response_later = (fun tr1 tr2 server payload -> ())
+  send_request = (fun tr client server request key_label -> True);
+  send_request_later = (fun tr1 tr2 client server request key_label -> ());
+  send_response = (fun tr server request response -> True);
+  send_response_later = (fun tr1 tr2 server request response -> ())
 }
 
 #push-options "--ifuel 1 --fuel 0"
@@ -147,26 +148,30 @@ let event_predicate_communication_layer_reqres
   event_predicate communication_reqres_event =
   fun tr prin e ->
     (match e with
-    | CommClientSendRequest client server payload key -> (
-      is_knowable_by (get_label tr key) tr payload /\
+    | CommClientSendRequest client server request key -> (
+      is_knowable_by (get_label tr key) tr request /\
       is_secret (comm_label client server) tr key /\
       key `has_usage tr` (AeadKey comm_layer_aead_tag empty) /\
-      (match parse a payload with
+      (match parse a request with
       | None -> False
-      | Some payload -> higher_layer_resreq_preds.send_request tr client server payload (get_label tr key))
+      | Some request -> higher_layer_resreq_preds.send_request tr client server request (get_label tr key))
     )
-    | CommServerReceiveRequest server payload key -> (
-      is_knowable_by (principal_label server) tr payload /\
-      (exists client. event_triggered tr client (CommClientSendRequest client server payload key) \/
-        is_publishable tr payload)
+    | CommServerReceiveRequest server request key -> (
+      is_knowable_by (principal_label server) tr request /\
+      (exists client. event_triggered tr client (CommClientSendRequest client server request key) \/
+        is_publishable tr request)
     )
-    | CommServerSendResponse server payload -> (
-      (match parse a payload with
+    | CommServerSendResponse server request response -> (
+      (match parse a response with
       | None -> False
-      | Some payload -> higher_layer_resreq_preds.send_response tr server payload)
+      | Some response -> (
+        match parse a request with
+        | None -> False
+        | Some request -> higher_layer_resreq_preds.send_response tr server request response)
+      )
     )
-    | CommClientReceiveResponse client server payload key -> (
-      event_triggered tr server (CommServerSendResponse server payload) \/
+    | CommClientReceiveResponse client server response key -> (
+      (exists request. event_triggered tr server (CommServerSendResponse server request response)) \/
       is_corrupt tr (principal_label client) \/ is_corrupt tr (principal_label server)
     )
     )
@@ -179,12 +184,12 @@ let request_response_event_preconditions #cinvs = {
   (default_comm_higher_layer_event_preds com_message_t) with
   send_conf = (fun tr client server (com_msg_t:com_message_t) ->
     match com_msg_t with
-    | RequestMessage {payload; key} -> (
-      event_triggered tr client (CommClientSendRequest client server payload key)
+    | RequestMessage {request; key} -> (
+      event_triggered tr client (CommClientSendRequest client server request key)
     )
     | _ -> False
   );
-  send_conf_later = (fun tr1 tr2 client server req_payload -> ()
+  send_conf_later = (fun tr1 tr2 client server msg -> ()
   )
 }
 #pop-options
