src/lib/communication/DY.Lib.Communication.RequestResponse.Properties.fst
@@ -1,0 +1,64 @@
+module DY.Lib.Communication.RequestResponse.Properties
+
+open Comparse
+open DY.Core
+open DY.Lib.Crypto.PKE.Split
+open DY.Lib.Crypto.Signature.Split
+open DY.Lib.Event.Typed
+open DY.Lib.State.PKI
+open DY.Lib.State.PrivateKeys
+open DY.Lib.State.Typed
+
+open DY.Lib.Communication.RequestResponse
+open DY.Lib.Communication.RequestResponse.Invariants
+
+#set-options "--fuel 0 --ifuel 0 --z3rlimit 10 --z3cliopt 'smt.qi.eager_threshold=100'"
+
+/// This module contains security properties that can be proven from the
+/// communication layer guarantees.
+
+(*** Authentication Security Properties ***)
+
+val server_authentication:
+  {|protocol_invariants|} ->
+  #a:Type -> {| parseable_serializeable bytes a |} ->
+  tr:trace -> i:timestamp ->
+  higher_layer_resreq_preds:comm_reqres_higher_layer_event_preds a ->
+  client:principal -> server:principal -> response:bytes -> key:bytes ->
+  Lemma
+  (requires
+    trace_invariant tr /\
+    has_communication_layer_reqres_event_predicates request_response_event_preconditions higher_layer_resreq_preds /\
+    event_triggered_at tr i client (CommClientReceiveResponse client server  response key)    
+  )
+  (ensures
+    (exists request. event_triggered (prefix tr i) server (CommServerSendResponse server request response)) \/
+    is_corrupt (prefix tr i) (principal_label client) \/ 
+    is_corrupt (prefix tr i) (principal_label server)
+  )
+let server_authentication #invs #a tr i higher_layer_resreq_preds client server response key = ()
+
+
+(*** Secrecy Security Property ***)
+
+val key_secrecy_client:
+  {|protocol_invariants|} ->
+  tr:trace ->
+  client:principal -> server:principal ->
+  key:bytes -> request:bytes -> response:bytes ->
+  Lemma
+  (requires
+    trace_invariant tr /\
+    has_communication_layer_state_predicates /\
+    attacker_knows tr key /\
+    (
+      (exists sid. state_was_set tr client sid (ClientSendRequest {server; request; key})) \/
+      (exists sid. state_was_set tr client sid (ClientReceiveResponse {server; response; key}))
+    )
+  )
+  (ensures
+    is_corrupt tr (principal_label client) \/ is_corrupt tr (principal_label server)
+  )
+let key_secrecy_client tr client server key request response =
+  attacker_only_knows_publishable_values tr key;
+  ()
